typeclass: prove termination of by_super

typeclass/typeclass_env_map_implScript.sml
@@ -1,9 +1,11 @@
 (* concrete data structures for implementing
 * instance map and type class map *)
 open HolKernel Parse boolLib bossLib dep_rewrite BasicProvers;
-
+open relationTheory set_relationTheory;
 open pairTheory optionTheory listTheory pred_setTheory finite_mapTheory
-open mlmapTheory mlstringTheory typeclass_tcexpTheory
+open mlmapTheory mlstringTheory balanced_mapTheory alistTheory;
+open miscTheory typeclass_unificationTheory
+typeclass_inference_commonTheory topological_sortTheory typeclass_tcexpTheory;
 
 val _ = new_theory "typeclass_env_map_impl";
 
@@ -56,11 +58,342 @@ Definition add_instance_def:
           | _ => NONE)
 End
 
-(*
-Definition lookup_inst_map_type_pat_def:
-  lookup_inst_map_type_pat (m:instinfo_impl) cl ty =
-  (ARB:(type # instinfo_impl) list)
+(* check if there is cyclic superclass relation *)
+Definition superAList_def:
+  superAList cl_map =
+    MAP (λ(k,v). (k, v.super)) $ toAscList cl_map
 End
-*)
+
+Definition check_cl_map_no_cycles_def:
+  check_cl_map_no_cycles cl_map =
+    ¬has_cycle (superAList cl_map)
+End
+
+Theorem fmap_to_alist_MAP_KEYS:
+  INJ f (FDOM m) UNIV ⇒
+  set (fmap_to_alist (MAP_KEYS f m)) =
+    set (MAP (λ(k,v). (f k,v)) $ fmap_to_alist m)
+Proof
+  Induct_on `m` >>
+  rw[] >>
+  `INJ f (FDOM m) UNIV`
+  by (
+    drule_then irule INJ_SUBSET >>
+    simp[]
+  ) >>
+  drule_then (fn t => simp[t]) MAP_KEYS_FUPDATE >>
+  fs[EXTENSION,LAMBDA_PROD,GSYM PFORALL_THM] >>
+  rpt gen_tac >>
+  simp[MEM_MAP,MEM_fmap_to_alist,
+    LAMBDA_PROD,GSYM PEXISTS_THM,FLOOKUP_UPDATE] >>
+  iff_tac
+  >- (
+    IF_CASES_TAC
+    >- (
+      rw[] >>
+      irule_at (Pos hd) EQ_REFL >>
+      simp[]) >>
+    rw[MEM_MAP] >>
+    pairarg_tac >>
+    fs[] >>
+    irule_at (Pos hd) EQ_REFL >>
+    fs[FDOM_FLOOKUP,FAPPLY_FUPDATE_THM] >>
+    IF_CASES_TAC >>
+    fs[FLOOKUP_DEF]) >>
+  fs[MEM_MAP,FAPPLY_FUPDATE_THM,LAMBDA_PROD,
+    GSYM PEXISTS_THM] >>
+  rw[]
+  >- (
+    IF_CASES_TAC >>
+    fs[INJ_DEF] >>
+    spose_not_then kall_tac >>
+    pop_assum mp_tac >>
+    simp[]) >>
+  irule_at (Pos hd) EQ_REFL >>
+  IF_CASES_TAC >>
+  fs[FLOOKUP_DEF]
+QED
+
+Triviality set_MAP_SINGLE_FST_EQ:
+  (∀x y. f x = f y ⇔ x = y) ∧
+  set (MAP f x) = set (MAP f y) ⇒
+  set x = set y
+Proof
+  simp[LIST_TO_SET_MAP] >>
+  metis_tac[IMAGE_11]
+QED
+
+Triviality set_MAP_key_EQ:
+  set (MAP (λ(k,v). ({k},v)) x) = set (MAP (λ(k,v). ({k},v)) y) ⇒
+  set x = set y
+Proof
+  qpat_abbrev_tac `f=(λ(k,v). ({k},v))` >>
+  strip_tac >>
+  drule_at_then (Pos last) irule set_MAP_SINGLE_FST_EQ >>
+  rw[Abbr`f`,EQ_IMP_THM] >>
+  ntac 2 (pairarg_tac >> fs[])
+QED
+
+Theorem mlmap_toAscList:
+  map_ok (m:('a,'b) map) ⇒
+  SORTED (λ(x,y) (x',y'). (cmp_of m) x x' = Less) (toAscList m) ∧
+  (set (toAscList m)) =
+    set (fmap_to_alist (
+      (to_fmap: ('a,'b) map -> ('a |-> 'b)) m))
+Proof
+  Cases_on `m` >>
+  simp[map_ok_def,mlmapTheory.toAscList_def,cmp_of_def] >>
+  strip_tac >>
+  drule_then assume_tac comparisonTheory.TotOrder_imp_good_cmp >>
+  drule_all balanced_mapTheory.toAscList_thm >>
+  rw[] >>
+  drule_then assume_tac to_fmap_thm >>
+  drule_then assume_tac TotOrd_key_set >>
+  fs[lift_key_def,GSYM LIST_TO_SET_MAP,MAP_KEYS_def] >>
+  irule set_MAP_key_EQ >>
+  qmatch_goalsub_abbrev_tac `MAP _ (fmap_to_alist m)` >>
+  `INJ (λx. {x}) (FDOM m) UNIV` by simp[INJ_DEF] >>
+  drule fmap_to_alist_MAP_KEYS >>
+  rw[]
+QED
+
+Triviality ALL_DISTINCT_superAList:
+  map_ok cl_map ⇒
+  ALL_DISTINCT (MAP FST $ superAList cl_map)
+Proof
+  rw[superAList_def,map_fst] >>
+  simp[mlmapTheory.MAP_FST_toAscList]
+QED
+
+Triviality super_reachable_EQ_TC_depends_on_weak:
+  map_ok cl_map ⇒
+  super_reachable (to_class_map cl_map) =
+    TC_depends_on_weak (superAList cl_map)
+Proof
+  rw[super_reachable_def,TC_depends_on_weak_def] >>
+  AP_TERM_TAC >>
+  rw[FUN_EQ_THM,superAList_def,map_fst,depends_on1_def] >>
+  fs[to_class_map_def,FLOOKUP_FMAP_MAP2,FMAP_MAP2_THM,PULL_EXISTS] >>
+  drule_then strip_assume_tac mlmap_toAscList >>
+  gvs[ALOOKUP_MAP,PULL_EXISTS,EXTENSION] >>
+  rw[EQ_IMP_THM]
+  >- (
+    drule_then assume_tac $
+      cj 2 mlmapTheory.MAP_FST_toAscList >>
+    drule_then assume_tac ALOOKUP_ALL_DISTINCT_MEM >>
+    drule_then strip_assume_tac mlmap_toAscList >>
+    fs[EXTENSION] >>
+    metis_tac[]
+  ) >>
+  drule_then assume_tac ALOOKUP_MEM >>
+  drule_then assume_tac $ cj 2 mlmap_toAscList >>
+  fs[EXTENSION]
+QED
+
+Theorem check_cl_map_no_cycles_IMP_super_no_cycles:
+  map_ok cl_map ∧
+  check_cl_map_no_cycles cl_map ⇒
+  super_no_cycles $ to_class_map cl_map
+Proof
+  rw[super_no_cycles_def] >>
+  drule_all_then assume_tac
+    super_reachable_EQ_TC_depends_on_weak >>
+  drule_then assume_tac ALL_DISTINCT_superAList >>
+  drule_then assume_tac has_cycle_correct2 >>
+  fs[check_cl_map_no_cycles_def]
+QED
+
+(* Similar to how it is implemented in
+ * "Typing Haskell in Haskell" by Mark P. Jones *)
+Theorem TC_flip:
+  ∀x y. TC R x y ⇒ TC (flip R) y x
+Proof
+  Induct_on `TC` >>
+  rw[]
+  >- 
+    (irule $ cj 1 relationTheory.TC_RULES >>
+    simp[]) >>
+  irule $ cj 2 relationTheory.TC_RULES >>
+  metis_tac[]
+QED
+
+Theorem WF_PULL_lift:
+  ∀P f R g R'. 
+  (!x. P (f x) ⇒ WF (R (f x))) ⇒
+  (∀x y. R' x y ⇒ P (f x) ∧ f x = f y ∧ R (f x) (g x) (g y)) ⇒
+  WF R'
+Proof
+  rw[WF_DEF] >>
+  reverse $ Cases_on `∃w'. P (f w') ∧ B w'`
+  >- (
+    fs[] >>
+    metis_tac[]) >>
+  rw[] >>
+  first_x_assum drule >>
+  qpat_x_assum `B w` kall_tac >>
+  rw[PULL_EXISTS] >>
+  first_x_assum $ qspec_then
+    `\x. ∃y. x = g y ∧ B y ∧ P (f y) ∧ f y = f w'` assume_tac >>
+  fs[PULL_EXISTS] >>
+  first_x_assum (dxrule_then dxrule) >>
+  rw[] >>
+  first_assum $ irule_at (Pos hd) >>
+  rw[] >>
+  last_x_assum drule >>
+  rw[] >>
+  gvs[]
+QED
+
+(* everything in the super list must be in the map *)
+(* ∧ mlmap$lookup cl_map c ≠ NONE ∧
+(∀cl info s.
+  lookup cl_map cl = SOME info ∧
+  MEM s info.super ⇒
+  mlmap$lookup cl_map s ≠ NONE) *)
+
+Theorem by_super_aux_terminate:
+  ∃R. WF R ∧
+       ∀visited t c cl_map clinfo sup visited'.
+         (map_ok cl_map ∧ check_cl_map_no_cycles cl_map) ∧
+         lookup cl_map c = SOME clinfo ∧ MEM sup clinfo.super ∧
+         lookup visited' sup = NONE ⇒
+         R (cl_map,visited',sup,t) (cl_map,visited,c,t)
+Proof
+  qexists
+  `(λ(cl_map,visited,sup,t) (cl_map',visited',c,t').
+    cl_map = cl_map' ∧ map_ok cl_map ∧
+    check_cl_map_no_cycles cl_map ∧
+    ∃info. lookup cl_map c = SOME info ∧
+      MEM sup info.super)` >>
+   rw[] >>
+   qspecl_then [
+     `\x. map_ok x ∧ check_cl_map_no_cycles x`,
+     `FST`,
+     `\x sup c. ∃info. lookup x c = SOME info ∧
+       MEM sup info.super`,
+       `λ(cl_map,visited,c,t). c`]
+     irule WF_PULL_lift >>
+   reverse $ rw[]
+   >- (
+    PairCases_on `x` >>
+    fs[] >>
+    rename1 `lookup cl_map` >>
+    `WF (reln_to_rel (rel_to_reln
+      (λsup c. ∃info. lookup cl_map c = SOME info ∧
+        MEM sup info.super)))`
+    suffices_by (
+      PURE_REWRITE_TAC[reln_rel_conv_thms] >>
+      simp[]) >>
+    irule acyclic_WF >>
+    simp[acyclic_def,rel_to_reln_def] >>
+    simp[reln_rel_conv_thms,reln_to_rel_def,
+      rel_to_reln_def] >>
+    conj_tac
+    >- (
+      rpt strip_tac >>
+      drule_all
+        check_cl_map_no_cycles_IMP_super_no_cycles >>
+      simp[super_no_cycles_def] >>
+      simp[super_reachable_def,to_class_map_def,
+        PULL_EXISTS,FLOOKUP_FMAP_MAP2] >>
+      drule TC_flip >>
+      simp[combinTheory.C_DEF,
+        GSYM mlmapTheory.lookup_thm] >>
+      metis_tac[]
+    ) >>
+    qexists
+      `{c | ∃x. lookup cl_map c = SOME x} ∪
+      BIGUNION (IMAGE (\info. set info.super) $
+      {info | ?c. lookup cl_map c = SOME info})` >>
+    rw[]
+    >- simp[mlmapTheory.lookup_thm,flookup_thm]
+    >- (
+      irule IMAGE_FINITE >>
+      `{info | ?c. mlmap$lookup cl_map c = SOME info} =
+        FRANGE (to_fmap cl_map)`
+      by simp[mlmapTheory.lookup_thm,EXTENSION,
+        IN_FRANGE,flookup_thm] >>
+      simp[])
+    >- simp[FINITE_LIST_TO_SET]
+    >- (
+      irule SUBSET_TRANS >>
+      irule_at (Pos last) $ cj 2 SUBSET_UNION >>
+      simp[mlmapTheory.lookup_thm,BIGUNION,
+        RDOM_DEF,SUBSET_DEF,IN_DEF] >>
+      metis_tac[]
+    )
+    >- (
+      irule SUBSET_TRANS >>
+      irule_at (Pos last) $ cj 1 SUBSET_UNION >>
+      rw[RRANGE,SUBSET_DEF,IN_DEF] >>
+      metis_tac[])
+   ) >>
+   ntac 2 (pairarg_tac >> fs[]) >>
+   metis_tac[]
+QED
+
+(* use map to store what super classes have been visited *)
+Definition by_super_aux_def:
+  by_super_aux cl_map visited c t =
+  if map_ok cl_map ∧ check_cl_map_no_cycles cl_map
+  then
+    case mlmap$lookup cl_map c of
+      | NONE => visited
+      | SOME clinfo =>
+        FOLDL  (λvisited sup.
+        case lookup visited sup of
+          | SOME _ => visited
+          | NONE => by_super_aux cl_map visited sup t)
+          (mlmap$insert visited c t)
+        clinfo.super
+  else visited (* should never happen *)
+Termination
+  metis_tac[by_super_aux_terminate]
+End
+
+Definition by_super_def:
+  by_super cl_map (c,t) =
+    by_super_aux cl_map (empty mlstring$compare) c t
+End
+
+Theorem by_super_thm:
+  map_ok cl_map ∧ check_cl_map_no_cycles cl_map ⇒
+  (mlmap$lookup (by_super cl_map (c,t)) s = SOME v ⇔
+    (v = t ∧ super_reachable (to_class_map cl_map) c s))
+Proof
+  rw[by_super_def] >>
+
+QED
+
+
+(* return a list of goals that the type has to satisfy in order
+* to satisfy c *)
+Definition apply_pred:
+  apply_pred m (cl,v) = OPTION_MAP (λt. (cl,t)) (FLOOKUP m v)
+End
+
+Definition by_inst_def:
+  byInst inst_map c t =
+  OPTION_BIND (lookup inst_map c) (λinstl.
+    let l  =
+      FILTER (λ(m,inst_info). IS_SOME m) $
+      MAP (λ(t',inst_info). (specialize t t',inst_info)) instl
+    in
+      if LENGTH l = 1
+      then
+        (case HD l of
+          (SOME m,inst_info) =>
+            OPT_MMAP (apply_pred m) inst_info.cstr)
+      else NONE)
+End
+
+Definition entail_def:
+  entail cl_map inst_map ps (c,t) = ANY (MEM (c,t)) (MAP (by_super
+  cl_map) ps) ∨
+  case by_inst inst_map c t of
+    | NONE => F
+    | SOME qs => ALL (entail cl_map inst_map ps) qs
+End
+
 
 val _ = export_theory();
