typeclass/typing/typeclass_kindCheckScript.sml
@@ -17,41 +17,41 @@ End
 
 Inductive kind_wf:
 [~Prim:]
-  ∀cdb vdb t. kind_wf cdb vdb kindType (Atom $ PrimTy t)
+  ∀t. kind_wf cdb vdb kindType (Atom $ PrimTy t)
 [~Exception:]
-  ∀cdb vdb. kind_wf cdb vdb kindType (Atom Exception)
+  kind_wf cdb vdb kindType (Atom Exception)
 [~VarTypeCons:]
-   ∀cdb vdb v.
-      kind_wf cdb vdb (vdb v) (Atom $ VarTypeCons v)
+  ∀v k.
+    vdb v = SOME k ⇒
+    kind_wf cdb vdb k (Atom $ VarTypeCons v)
 [~TyConsINL:]
-   ∀cdb vdb c.
-      kind_wf cdb vdb (cdb c) (Atom $ TypeCons (INL c))
+  ∀c k.
+    cdb c = SOME k ⇒
+    kind_wf cdb vdb k (Atom $ TypeCons (INL c))
 [~TyConsFunction:]
-   ∀cdb vdb.
-      kind_wf cdb vdb (kindArrow kindType $ kindArrow kindType kindType)
-        (Atom $ TypeCons (INR Function))
+   kind_wf cdb vdb
+     (kindArrow kindType $ kindArrow kindType kindType)
+     (Atom $ TypeCons (INR Function))
 [~TypeConsArray:]
-   ∀cdb vdb.
-      kind_wf cdb vdb (kindArrow kindType kindType)
-        (Atom $ TypeCons (INR Array))
+   kind_wf cdb vdb (kindArrow kindType kindType)
+     (Atom $ TypeCons (INR Array))
 [~TypeConsM:]
-   ∀cdb vdb.
-      kind_wf cdb vdb (kindArrow kindType kindType)
-        (Atom $ TypeCons (INR M))
+   kind_wf cdb vdb (kindArrow kindType kindType)
+     (Atom $ TypeCons (INR M))
 [~TypeConsTuple:]
-   ∀cdb vdb n.
-      kind_wf cdb vdb (kind_arrows (GENLIST (K kindType) n) kindType)
-        (Atom $ TypeCons (INR $ Tuple n))
+   ∀n.
+     kind_wf cdb vdb (kind_arrows (GENLIST (K kindType) n) kindType)
+       (Atom $ TypeCons (INR $ Tuple n))
 [~Cons:]
-   ∀cdb vdb k1 k2 t1 t2.
-      kind_wf cdb vdb (kindArrow k1 k2) t1 /\
-      kind_wf cdb vdb k1 t2 ==>
-        kind_wf cdb vdb k2 (Cons t1 t2)
+   ∀k1 k2 t1 t2.
+     kind_wf cdb vdb (kindArrow k1 k2) t1 ∧
+     kind_wf cdb vdb k1 t2 ⇒
+       kind_wf cdb vdb k2 (Cons t1 t2)
 End
 
-(* predicate to check if the predicated type is well-kinded *)
-Definition kind_ok_def:
-  kind_ok cldb cdb vdb (Pred cls ty) =
+(* predicate to check if a predicated type is well-kinded *)
+Definition pred_type_kind_ok_def:
+  pred_type_kind_ok cldb cdb vdb (Pred cls ty) =
     (kind_wf cdb vdb kindType ty ∧
     ∀v cl. MEM (cl,v) cls ==>
       kind_wf cdb vdb (cldb cl) v)
@@ -62,14 +62,4 @@ Definition kind_to_arities_def:
   (kind_to_arities kindType = 0)
 End
 
-(*
-Definition ns_cns_kind_def:
-  ns_cns_kind (exndef: exndef, tdefs : typedefs) =
-    set (MAP (λ(cn,ts). cn, _ ts) exndef) INSERT
-    {(«True», kindType); («False», kindType)} (* Booleans considered built-in *) INSERT
-    set (_ tdefs)
-    (* there could be mutual-recursive types and
-    * needs to do kind inference at the same time *)
-End
-*)
 val _ = export_theory();
