typeclass/typing/typeclass_specializeScript.sml
@@ -1,0 +1,36 @@
+(* Implement specialization for predicated types using unification *)
+
+open HolKernel Parse boolLib bossLib BasicProvers dep_rewrite;
+open pairTheory arithmeticTheory integerTheory stringTheory optionTheory
+     pred_setTheory relationTheory listTheory alistTheory finite_mapTheory;
+open typeclass_unificationTheory typeclass_typesTheory;
+(* typeclass_typingTheory *)
+open typeclass_inference_commonTheory;
+
+val _ = new_theory "typeclass_specialization";
+
+val _ = monadsyntax.enable_monadsyntax()
+val _ = monadsyntax.enable_monad "option"
+
+(* to avoid variable name collision get the max variable index *)
+Definition:
+End
+
+Definition VarType_to_CVar_def:
+  (VarType_to_CVar (iAtom (VarTypeCons v)) = iCVar v) ∧
+  (VarType_to_CVar (iCons i1 i2) = iCons (VarType_to_CVar i1) (VarType_to_CVar i2)) ∧
+  (VarType_to_CVar (iCVar n) = iAtom ) ∧ (* this should never happend *)
+  (VarType_to_CVar i = i)
+End
+
+Definition specialize_def:
+  specialize t t' = (?ts. tsubst ts t = t')
+End
+
+Definition specialize_impl_def:
+  specialize_impl t t' = pure_unify FEMPTY (VarType_to_CVar (itype_of t)) (itype_of t')
+End
+
+
+
+val _ = export_theory();
