typeclass/typing/typeclass_typesScript.sml
@@ -44,37 +44,9 @@ End
 
 Overload Unit = ``Atom $ TypeCons (INR $ Tuple 0)``;
 Overload TypeVar = ``\x. Atom (VarTypeCons x)``;
+Overload UserType = ``\x. Atom (TypeCons $ INL x)``;
 Type type_scheme[pp] = ``:num # type``;
 Type PredType_scheme[pp] = ``:num # PredType``;
-
-(*
-  A type definition is an arity and a collection of constructor definitions.
-  Each constructor definition is a name and a type scheme for its arguments
-  (closed wrt the type definition arity).
-
-  Like CakeML, use numbers to refer to types - known typedefs represented as
-    : typedef list
-  We could instead have:
-    : (string # typedef) list     or     : string |-> typedef     etc.
-  Unlike CakeML, we group constructors by their type (i.e. group siblings).
-
-  E.g. the type definitions for Maybe and List might look like:
-  [
-    (1, [ ("Nothing", []) ; ("Just", [Var 0]) ]);
-    (1, [ ("Nil", []) ; ("Cons", [Var 0; TypeCons 1 [Var 0]]) ])
-  ]
-
-  The exception definition is a list of constructors associated to (closed)
-  argument types.
-
-  Together, the exception definition and a collection of type definitions form
-  our typing namespace.
-*)
-
-(* TODO make finite maps *)
-Type typedef[pp] = ``:num # ((mlstring # type list) list)``;
-Type typedefs[pp] = ``:typedef list``;
-Type exndef[pp] = ``:(mlstring # type list) list``;
 
 Definition collect_type_vars_def:
   (collect_type_vars (Cons t1 t2) =
@@ -82,5 +54,117 @@ Definition collect_type_vars_def:
   (collect_type_vars (Atom $ VarTypeCons v) = {v}) /\
   (collect_type_vars _ = {})
 End
+
+(********** Substitutions and shifts **********)
+
+Definition subst_db_def:
+  (subst_db skip ts (Atom (VarTypeCons v)) =
+    if skip ≤ v ∧ v < skip + LENGTH ts
+      then EL (v - skip) ts 
+    else if skip ≤ v
+      then Atom (VarTypeCons $ v - LENGTH ts)
+    else
+      Atom (VarTypeCons v)) ∧
+  (subst_db skip ts (Atom a) = Atom a) ∧
+  subst_db skip ts (Cons t1 t2) =
+    Cons (subst_db skip ts t1) (subst_db skip ts t2)
+End
+
+Definition shift_db_def:
+  (shift_db skip n (Atom (VarTypeCons db)) =
+    if skip ≤ db
+      then Atom (VarTypeCons $ db + n)
+      else Atom (VarTypeCons db)) ∧
+  (shift_db skip n (Atom a) = Atom a) ∧
+  shift_db skip n (Cons t1 t2) =
+    Cons (shift_db skip n t1) (shift_db skip n t2)
+End
+
+Overload subst_db_scheme =
+  ``λn ts (vars,scheme).
+      (vars, subst_db (n + vars) (MAP (shift_db 0 vars) ts) scheme)``;
+Overload shift_db_scheme =
+  ``λskip shift (vars,scheme).
+      (vars, shift_db (skip + vars) shift scheme)``;
+Overload tsubst = ``subst_db 0``;
+Overload tshift = ``shift_db 0``;
+Overload tshift_scheme = ``λn (vars,scheme). (vars, shift_db vars n scheme)``;
+Overload tshift_env = ``λn. MAP (λ(x,scheme). (x, tshift_scheme n scheme))``;
+
+Definition Functions_def:
+  Functions [] t = t ∧
+  Functions (at::ats) t =
+    Cons
+      (Cons (Atom $ TypeCons $ INR Function) at) $
+      Functions ats t
+End
+
+
+(* What's the proper way to do this *)
+Definition generalise_def:
+  generalise db (avoid : num_set) s (DBVar n) = (0n, s, DBVar n) ∧
+  generalise db avoid s (PrimTy p) = (0, s, PrimTy p) ∧
+  generalise db avoid s  Exception = (0, s, Exception) ∧
+
+  generalise db avoid s (TypeCons id ts) = (
+    let (n, s', ts') = generalise_list db avoid s ts in (n, s', TypeCons id ts')) ∧
+
+  generalise db avoid s (Tuple ts) = (
+    let (n, s', ts') = generalise_list db avoid s ts in (n, s', Tuple ts')) ∧
+
+  generalise db avoid s (Function t1 t2) = (
+    let (n1, s', t1') = generalise db avoid s t1 in
+    let (n2, s'', t2') = generalise (db + n1) avoid s' t2 in
+    (n1 + n2, s'', Function t1' t2')) ∧
+
+  generalise db avoid s (Array t) = (
+    let (n, s', t') = generalise db avoid s t in (n, s', Array t')) ∧
+
+  generalise db avoid s (M t) = (
+    let (n, s', t') = generalise db avoid s t in (n, s', M t')) ∧
+
+  generalise db avoid s (CVar c) = (
+    if lookup c avoid = NONE then (
+      case FLOOKUP s c of
+      | SOME n => (0, s, DBVar n)
+      | NONE => (1, s |+ (c,db), DBVar db))
+    else (0, s, CVar c)) ∧
+
+  generalise_list db avoid s [] = (0, s, []) ∧
+  generalise_list db avoid s (t::ts) =
+    let (n, s', t') = generalise db avoid s t in
+    let (ns, s'', ts') = generalise_list (db + n) avoid s' ts in
+    (n + ns, s'', t'::ts')
+End
+
+
+Definition max_db_def:
+  max_db (Cons t1 t2) = MAX (max_db t1) (max_db t2) ∧
+  max_db (Atom (VarTypeCons v)) = 1 + v ∧
+  max_db (Atom a) = 0
+End
+
+Definition to_scheme_def:
+  to_scheme db avoid s (Cons t1 t2) =
+    let (n,s',t1') = to_scheme db avoid s t1 in
+    let (n',s'',t2') = to_scheme (db + n) avoid s t2 in
+    (n+n',s'',Cons t1' t2') ∧
+  to_scheme db avoid s (Atom (VarTypeCons v)) =
+    if lookup v avoid = NONE
+    then (0,s,Atom (VarTypeCons v))
+    else (1,s,Atom (VarTypeCons db))
+End
+
+(******************** Properties of types ********************)
+
+Definition freetyvars_ok_def:
+  (freetyvars_ok n (Atom (VarTypeCons v)) = (v < n)) ∧
+  (freetyvars_ok n (Atom a) = T) ∧
+  (freetyvars_ok n (Cons t1 t2) =
+    (freetyvars_ok n t1 ∧ freetyvars_ok n t2))
+End
+
+Overload freetyvars_ok_scheme =
+  ``λn (vars,scheme). freetyvars_ok (n + vars) scheme``;
 
 val _ = export_theory();
