typeclass/typing/typeclass_typingScript.sml
@@ -1,9 +1,38 @@
 open HolKernel Parse boolLib bossLib BasicProvers;
 open pairTheory arithmeticTheory integerTheory stringTheory optionTheory
      listTheory alistTheory;
-open typeclass_typesTheory typeclass_tcexpTheory pure_configTheory;
+open typeclass_typesTheory typeclass_tcexpTheory
+typeclass_kindCheckTheory pure_configTheory;
 
 val _ = new_theory "typeclass_typing";
+
+(*
+  A type definition is an arity and a collection of constructor definitions.
+  Each constructor definition is a name and a type scheme for its arguments
+  (closed wrt the type definition arity).
+
+  Like CakeML, use numbers to refer to types - known typedefs represented as
+    : typedef list
+  We could instead have:
+    : (string # typedef) list     or     : string |-> typedef     etc.
+  Unlike CakeML, we group constructors by their type (i.e. group siblings).
+
+  E.g. the type definitions for Maybe and List might look like:
+  [
+    (1, [ ("Nothing", []) ; ("Just", [Var 0]) ]);
+    (1, [ ("Nil", []) ; ("Cons", [Var 0; TypeCons 1 [Var 0]]) ])
+  ]
+
+  The exception definition is a list of constructors associated to (closed)
+  argument types.
+
+  Together, the exception definition and a collection of type definitions form
+  our typing namespace.
+*)
+
+Type typedef[pp] = ``:Kind list # ((mlstring # type list) list)``;
+Type typedefs[pp] = ``:typedef list``;
+Type exndef[pp] = ``:(mlstring # type list) list``;
 
 (* CakeML assumes the following initial namespace:
       Exceptions: 0 -> Bind, 1 -> Chr, 2 -> Div, 3 -> Subscript
@@ -14,22 +43,17 @@ val _ = new_theory "typeclass_typing";
       Exception: 0 -> Subscript
       Types: 0 -> List
 *)
-
+(* TODO: should we change this to kind instead of just arities *)
+(* somthing like f [] and f Int ??*)
 Definition initial_namespace_def:
   initial_namespace : exndef # typedefs = (
     [«Subscript»,[]],
-    [1, [ («[]»,[]) ; («::»,[VarTypeCons 0 []; TypeCons (INL 0) [VarTypeCons 0 []]]) ]]
+    [[kindType],[(«[]»,[]);
+      («::», [TypeVar 0; Cons (UserType 0) (TypeVar 0)])]]
   )
 End
 
-Definition initial_kindmap_def:
-  initial_kindmap (INR Function) = kind_arrows [kindType;kindType] kindType ∧
-  initial_kindmap (INR (Tuple n)) = kind_arrows (GENLIST (K kindType) n)
-  kindType ∧
-  initial_kindmap (INR Array) = kindArrow kindType kindType ∧
-  initial_kindmap (INR M) = kindArrow kindType kindType
-End
-
+(* TODO: Why do we need this? *)
 (* Constructor names and their arities defined by a namespace *)
 Definition ns_cns_arities_def:
   ns_cns_arities (exndef : exndef, tdefs : typedefs) =
@@ -46,98 +70,13 @@ Definition cns_arities_ok_def:
     (∃cn_ars'. cn_ars' ∈ ns_cns_arities ns ∧ cn_ars ⊆ cn_ars')
 End
 
-Definition apply_rest_def:
-  apply_rest (TypeCons n tcs) rest = TypeCons n (tcs ++ rest) ∧
-  apply_rest (VarTypeCons n tcs) rest = VarTypeCons n (tcs ++ rest)
-End
-
-(********** Substitutions and shifts **********)
-
-Definition subst_db_def:
-  subst_db skip ts (PrimTy p) = PrimTy p ∧
-  subst_db skip ts  Exception = Exception ∧
-  subst_db skip ts (TypeCons n tcs) = TypeCons n (MAP (subst_db skip ts) tcs) ∧
-  subst_db skip ts (VarTypeCons v tcs) = (
-    if skip <= v ∧ v < skip + LENGTH ts then
-      apply_rest (EL (v - skip) ts) (MAP (subst_db skip ts) tcs)
-    else if skip <= v then
-      VarTypeCons (v - LENGTH ts) (MAP (subst_db skip ts) tcs)
-    else VarTypeCons v (MAP (subst_db skip ts) tcs))
-Termination
-  WF_REL_TAC `measure (type_size o SND o SND)` >> rw[fetch "pure_types" "type_size_def"] >>
-  rename1 `MEM _ ts` >> Induct_on `ts` >> rw[fetch "pure_types" "type_size_def"] >> gvs[]
-End
-
-Definition shift_db_def:
-  shift_db skip n (PrimTy p) = PrimTy p ∧
-  shift_db skip n  Exception = Exception ∧
-  shift_db skip n (TypeCons tn tcs) = TypeCons tn (MAP (shift_db skip n) tcs) ∧
-  shift_db skip n (VarTypeCons tn tcs) = (if skip <= tn
-    then VarTypeCons (tn + n) (MAP (shift_db skip n) tcs)
-    else VarTypeCons tn (MAP (shift_db skip n) tcs))
-Termination
-  WF_REL_TAC `measure (type_size o SND o SND)` >> rw[fetch "pure_types" "type_size_def"] >>
-  rename1 `MEM _ ts` >> Induct_on `ts` >> rw[fetch "pure_types" "type_size_def"] >> gvs[]
-End
-
-Overload subst_db_scheme =
-  ``λn ts (vars,scheme).
-      (vars, subst_db (n + vars) (MAP (shift_db 0 vars) ts) scheme)``;
-Overload shift_db_scheme =
-  ``λskip shift (vars,scheme).
-      (vars, shift_db (skip + vars) shift scheme)``;
-Overload tsubst = ``subst_db 0``;
-Overload tshift = ``shift_db 0``;
-Overload tshift_scheme = ``λn (vars,scheme). (vars, shift_db vars n scheme)``;
-Overload tshift_env = ``λn. MAP (λ(x,scheme). (x, tshift_scheme n scheme))``;
-
-Definition Functions_def:
-  Functions [] t = t ∧
-  Functions (at::ats) t = TypeCons (INR Function) [at;Functions ats t]
-End
-
-
-(******************** Properties of types ********************)
-
-Definition freetyvars_ok_def:
-  freetyvars_ok n (PrimTy p) = T ∧
-  freetyvars_ok n  Exception = T ∧
-  freetyvars_ok n (TypeCons c ts) = EVERY (freetyvars_ok n) ts ∧
-  freetyvars_ok n (VarTypeCons v ts) = (v < n ∧ EVERY (freetyvars_ok n) ts)
-Termination
-  WF_REL_TAC `measure (type_size o SND)` >> rw[fetch "pure_types" "type_size_def"] >>
-  rename1 `MEM _ ts` >> Induct_on `ts` >> rw[fetch "pure_types" "type_size_def"] >> gvs[]
-End
-
-Overload freetyvars_ok_scheme =
-  ``λn (vars,scheme). freetyvars_ok (n + vars) scheme``;
-
-(* Does a type only contain defined constructors, and non-nullary functions? *)
-(* replace with kind check *)
 Definition type_wf_def:
-  type_wf (typedefs : typedefs) (TypeVar n) = T ∧
-  type_wf typedefs (PrimTy pty) = T ∧
-  type_wf typedefs  Exception = T ∧
-  type_wf typedefs (TypeCons (SOME id) tyargs) = (
-    EVERY (type_wf typedefs) tyargs ∧
-    ∃arity constructors.
-      (* Type definition exists: *)
-        oEL id typedefs = SOME (arity, constructors) ∧
-      (* And has correct arity: *)
-        LENGTH tyargs = arity) ∧
-  type_wf typedefs (TypeCons NONE ts) = (* Tuple *)
-    EVERY (type_wf typedefs) ts ∧
-  type_wf typedefs (VarTypeCons id tyargs) = (
-    EVERY (type_wf typedefs) tyargs ∧
-    (* TODO *)
-  ) ∧
-  type_wf typedefs (Function tf t) = (
-    type_wf typedefs t ∧ type_wf typedefs tf) ∧
-  type_wf typedefs (Array t) = type_wf typedefs t ∧
-  type_wf typedefs (M t) = type_wf typedefs t
-Termination
-  WF_REL_TAC `measure (type_size o SND)` >> rw[fetch "-" "type_size_def"] >>
-  rename1 `MEM _ ts` >> Induct_on `ts` >> rw[fetch "-" "type_size_def"] >> gvs[]
+  type_wf (typedefs : typedefs) t =
+    ∃vdb.
+      kind_wf
+      (λc. OPTION_MAP
+        (λks. kind_arrows (FST ks) kindType)
+        (oEL c typedefs)) vdb kindType t
 End
 
 Definition type_ok_def:
